Update Evaluation and Substitution files

theories/Evaluation.v
@@ -8,226 +8,195 @@ Wormholes's semantics are divided in three sub semantics:
 - evaluation transition <--
 - functional transition
 - temporal transition
-
-This file focuses on the evaluation transition which is a small step semantics with a call by value evaluation strategy.
 *)
 
 
 (** *** Definition *)
 
-Reserved Notation "k '⊨' t '⟼' t1" (at level 57, t custom wormholes, 
-                                                   t1 custom wormholes, no associativity).
-Reserved Notation "k '⊨' t '⟼⋆' t1" (at level 57, t custom wormholes, 
-                                                    t1 custom wormholes, no associativity).
-Reserved Notation "k '⊨' t '⊢' st '⟶' t1" (at level 57, t custom wormholes, 
-                                                         t1 custom wormholes, no associativity).
+Reserved Notation "'⊨' t '⟼' t1" (at level 57, t custom rsf, 
+                                                   t1 custom rsf, no associativity).
+Reserved Notation "'⊨' t '⟼⋆' t1" (at level 57, t custom rsf, 
+                                                    t1 custom rsf, no associativity).
+Reserved Notation "'⊨' t '⊢' st '⟶' t1" (at level 57, t custom rsf, 
+                                                         t1 custom rsf, no associativity).
 
-(** **** Small-step semantics
-
-  Evaluation transition is defined as we found in an stlc formalization with a slight difference. Indeed, we have an additional element
-  [lb]. This is the current level that are valid. It is required because of the definition of validity of terms and for a well use of the 
-  substitution in the [eT_appv] rule. 
-*)
-Inductive evaluate : nat -> Λ -> Λ -> Prop :=
-  | eT_appv   : forall lb x τ t v,
+Inductive evaluate : Λ -> Λ -> Prop :=
+  | eT_appv   : forall x τ t v,
                                   value(v) ->
                 (*-------------------------------------------- ET-Appv *)
-                    lb ⊨ ((\x:τ,t) v) ⟼ ([x:= v ~ lb ≤ 0] t)
+                    ⊨ ((\x:τ,t) v) ⟼ ([x:= v] t)
 
 
-  | eT_fix   : forall lb f τ t,
+  | eT_fix   : forall f τ t,
                 (*------------------------------------------------------------ ET-Fix *)
-                    lb ⊨ (Fix (\f:τ,t)) ⟼ ([f := (Fix (\f:τ,t)) ~ lb ≤ 0] t)
+                    ⊨ (Fix (\f:τ,t)) ⟼ ([f := (Fix (\f:τ,t))] t)
 
-  | eT_app1   : forall lb t1 t1' t2,
-                        lb ⊨ t1 ⟼ t1' -> 
+  | eT_app1   : forall t1 t1' t2,
+                        ⊨ t1 ⟼ t1' -> 
                 (*---------------------------- ET-App1 *)
-                    lb ⊨ (t1 t2) ⟼ (t1' t2)
+                    ⊨ (t1 t2) ⟼ (t1' t2)
 
-  | eT_app2   : forall lb v t t',
-                    value(v) -> lb ⊨ t ⟼ t' -> 
+  | eT_app2   : forall v t t',
+                    value(v) -> ⊨ t ⟼ t' -> 
                 (*------------------------------- ET-App2 *)
-                      lb ⊨ (v t) ⟼ (v t') 
+                      ⊨ (v t) ⟼ (v t') 
 
-  | eT_pair1  : forall lb t1 t1' t2,
-                        lb ⊨ t1 ⟼ t1' -> 
+  | eT_pair1  : forall t1 t1' t2,
+                        ⊨ t1 ⟼ t1' -> 
                 (*----------------------------- ET-Pair1 *)
-                    lb ⊨ ⟨t1,t2⟩ ⟼ ⟨t1',t2⟩
+                    ⊨ ⟨t1,t2⟩ ⟼ ⟨t1',t2⟩
 
-  | eT_pair2  : forall lb v t t',
-                    value(v) -> lb ⊨ t ⟼ t' -> 
+  | eT_pair2  : forall v t t',
+                    value(v) -> ⊨ t ⟼ t' -> 
                 (*------------------------------- ET-Pair2 *)
-                      lb ⊨ ⟨v,t⟩ ⟼ ⟨v,t'⟩ 
+                      ⊨ ⟨v,t⟩ ⟼ ⟨v,t'⟩ 
 
-  | eT_fst1   : forall lb t t',
-                      lb ⊨ t ⟼ t' -> 
+  | eT_fst1   : forall t t',
+                      ⊨ t ⟼ t' -> 
                 (*------------------------- ET-Fst1 *)
-                    lb ⊨ t.fst ⟼ t'.fst
+                    ⊨ t.fst ⟼ t'.fst
 
-  | eT_fstv   : forall lb v1 v2,
+  | eT_fstv   : forall v1 v2,
                     value(v1) -> value(v2) -> 
                 (*----------------------------- ET-Fstv *)
-                    lb ⊨ ⟨v1,v2⟩.fst ⟼ v1
+                    ⊨ ⟨v1,v2⟩.fst ⟼ v1
 
-  | eT_snd1   : forall lb t t',
-                        lb ⊨ t ⟼ t' -> 
+  | eT_snd1   : forall t t',
+                        ⊨ t ⟼ t' -> 
                 (*-------------------------- ET-Snd1 *)
-                    lb ⊨ t.snd ⟼ t'.snd
+                    ⊨ t.snd ⟼ t'.snd
 
-  | eT_sndv   : forall lb v1 v2,
+  | eT_sndv   : forall v1 v2,
                     value(v1) -> value(v2) -> 
                 (*----------------------------- ET-Sndv *)
-                    lb ⊨ ⟨v1,v2⟩.snd ⟼ v2
+                    ⊨ ⟨v1,v2⟩.snd ⟼ v2
                             
-  | eT_comp1  : forall lb t1 t1' t2,
-                            lb ⊨ t1 ⟼ t1' -> 
+  | eT_comp1  : forall t1 t1' t2,
+                            ⊨ t1 ⟼ t1' -> 
                 (*--------------------------------- ET-Comp1 *)
-                    lb ⊨ t1 >>> t2 ⟼ t1' >>> t2
+                    ⊨ t1 >>> t2 ⟼ t1' >>> t2
 
-  | eT_comp2  : forall lb v t t',
-                      value(v) -> lb ⊨ t ⟼ t' -> 
+  | eT_comp2  : forall v t t',
+                      value(v) -> ⊨ t ⟼ t' -> 
                 (*--------------------------------- ET-Comp2 *)
-                      lb ⊨ v >>> t ⟼ v >>> t'
+                      ⊨ v >>> t ⟼ v >>> t'
 
-  | eT_arr  : forall lb t t',
-                      lb ⊨ t ⟼ t' -> 
+  | eT_arr  : forall t t',
+                      ⊨ t ⟼ t' -> 
               (*------------------------- ET-Arr *)
-                  lb ⊨ arr(t) ⟼ arr(t')
+                  ⊨ arr(t) ⟼ arr(t')
 
-  | eT_first  : forall lb τ t t',
-                            lb ⊨ t ⟼ t' -> 
+  | eT_first  : forall τ t t',
+                            ⊨ t ⟼ t' -> 
                 (*--------------------------------- ET-First *)
-                    lb ⊨ first(τ:t) ⟼ first(τ:t')
+                    ⊨ first(τ:t) ⟼ first(τ:t')
 
-  | eT_wh1   :  forall lb i i' t,
-                                lb ⊨ i ⟼ i' -> 
-                (*----------------------------------------- ET-Wh1 *)
-                    lb ⊨ wormhole(i;t) ⟼ wormhole(i';t)
-
-  | eT_wh2   :  forall lb i t t',
-                    value(i) -> (S (S lb)) ⊨ t ⟼ t' -> 
-                (*----------------------------------------- ET-Wh2 *)
-                    lb ⊨ wormhole(i;t) ⟼ wormhole(i;t')
-
-where "k '⊨' t '⟼' t1" := (evaluate k t t1)
+where "'⊨' t '⟼' t1" := (evaluate t t1)
 .
 
 (** **** Multi transition step with fuel *)
-Inductive indexed : nat -> nat -> Λ -> Λ -> Prop :=
-  | index_refl : forall lb x, lb ⊨ x ⊢ 0 ⟶ x
-  | index_step : forall lb k x y z, lb ⊨ x ⟼ y -> lb ⊨ y ⊢ k ⟶ z -> lb ⊨ x ⊢(S k)⟶ z
-where "k '⊨' t '⊢' st '⟶' t1" := (indexed k st t t1)
+Inductive indexed : nat -> Λ -> Λ -> Prop :=
+  | index_refl : forall x, ⊨ x ⊢ 0 ⟶ x
+  | index_step : forall k x y z, ⊨ x ⟼ y -> ⊨ y ⊢ k ⟶ z -> ⊨ x ⊢(S k)⟶ z
+where "'⊨' t '⊢' st '⟶' t1" := (indexed st t t1)
 .
 
 (** **** Multi transition step *)
-Inductive multi : nat -> Λ -> Λ -> Prop :=
-  | multi_refl : forall k x, k ⊨ x ⟼⋆ x
-  | multi_step : forall k x y z, k ⊨ x ⟼ y -> k ⊨ y ⟼⋆ z -> k ⊨ x ⟼⋆ z
-where "k '⊨' t '⟼⋆' t1" := (multi k t t1).
+Inductive multi : Λ -> Λ -> Prop :=
+  | multi_refl : forall x, ⊨ x ⟼⋆ x
+  | multi_step : forall x y z, ⊨ x ⟼ y -> ⊨ y ⟼⋆ z -> ⊨ x ⟼⋆ z
+where "'⊨' t '⟼⋆' t1" := (multi t t1).
 
 Definition normal_form {X : Type} (R : relation X) (t : X) : Prop := not (exists t', R t t').
-Definition halts (k : nat)  (t : Λ) : Prop :=  exists t', k ⊨ t ⟼⋆ t' /\  value(t').
+Definition halts (t : Λ) : Prop :=  exists t', ⊨ t ⟼⋆ t' /\  value(t').
 
 #[export] Hint Constructors evaluate multi indexed : core.
 
 (** *** Lift semantics rules from evaluation to multi evaluation *)
 
-Lemma multi_var : forall k (x : variable), k ⊨ x ⟼⋆ x.
-Proof. intros k x; apply multi_refl. Qed.
+Lemma multi_var : forall (x : variable), ⊨ x ⟼⋆ x.
+Proof. intros x; apply multi_refl. Qed.
 
-Lemma multi_appv : forall k x t τ v, 
-  value(v) -> k ⊨ ((\x:τ, t) v) ⟼⋆ ([x := v ~ k ≤ 0] t).
+Lemma multi_appv : forall x t τ v, 
+  value(v) -> ⊨ ((\x:τ, t) v) ⟼⋆ ([x := v] t).
 Proof. 
-  intros k x t τ v Hv. apply multi_step with (y := <[[x := v ~ k ≤ 0] t]>); auto.
+  intros x t τ v Hv. apply multi_step with (y := <[[x := v] t]>); auto.
 Qed.
 
-Lemma multi_fix : forall k x t τ, 
-  k ⊨ (Fix (\x:τ, t)) ⟼⋆ ([x := (Fix (\x:τ, t)) ~ k ≤ 0] t).
+Lemma multi_fix : forall x t τ, 
+  ⊨ (Fix (\x:τ, t)) ⟼⋆ ([x := (Fix (\x:τ, t))] t).
 Proof. 
-  intros k x t τ. apply multi_step with (y := <[[x := (Fix (\x:τ, t)) ~ k ≤ 0] t]>); auto.
+  intros x t τ. apply multi_step with (y := <[[x := (Fix (\x:τ, t))] t]>); auto.
 Qed.
 
-Lemma multi_app1 : forall k t t' t2, k ⊨ t ⟼⋆ t' -> k ⊨ (t t2) ⟼⋆ (t' t2).
+Lemma multi_app1 : forall t t' t2, ⊨ t ⟼⋆ t' -> ⊨ (t t2) ⟼⋆ (t' t2).
 Proof. 
-  intros k t t' t2 HeT; induction HeT; subst; auto.
+  intros t t' t2 HeT; induction HeT; subst; auto.
   apply multi_step with <[y t2]>; auto.
 Qed.
 
-Lemma multi_app2 : forall k t t' t1, value(t1) -> k ⊨ t ⟼⋆ t' -> k ⊨ (t1 t) ⟼⋆ (t1 t').
+Lemma multi_app2 : forall t t' t1, value(t1) -> ⊨ t ⟼⋆ t' -> ⊨ (t1 t) ⟼⋆ (t1 t').
 Proof. 
-  intros k t t' t1 Hvt HeT; induction HeT; subst; auto.
+  intros t t' t1 Hvt HeT; induction HeT; subst; auto.
   apply multi_step with <[t1 y]>; auto.
 Qed.
 
-Lemma multi_pair1 : forall k t t' t2, k ⊨ t ⟼⋆ t' -> k ⊨ ⟨t,t2⟩ ⟼⋆ ⟨t',t2⟩.
+Lemma multi_pair1 : forall t t' t2, ⊨ t ⟼⋆ t' -> ⊨ ⟨t,t2⟩ ⟼⋆ ⟨t',t2⟩.
 Proof.
-  intros k t t' t2 HeT; induction HeT; subst; auto.
+  intros t t' t2 HeT; induction HeT; subst; auto.
   apply multi_step with <[⟨y,t2⟩]>; auto. 
 Qed.
 
-Lemma multi_pair2 : forall k t t' t1, value(t1) -> k ⊨ t ⟼⋆ t' -> k ⊨ ⟨t1,t⟩ ⟼⋆ ⟨t1,t'⟩.
+Lemma multi_pair2 : forall t t' t1, value(t1) -> ⊨ t ⟼⋆ t' -> ⊨ ⟨t1,t⟩ ⟼⋆ ⟨t1,t'⟩.
 Proof.
-  intros k t t' t1 Hvt HeT; induction HeT; subst; auto.
+  intros t t' t1 Hvt HeT; induction HeT; subst; auto.
   apply multi_step with <[⟨t1,y⟩]>; auto. 
 Qed.
 
-Lemma multi_fstv : forall k t1 t2, value(t1) -> value(t2) -> k ⊨ ⟨t1,t2⟩.fst ⟼⋆ t1.
+Lemma multi_fstv : forall t1 t2, value(t1) -> value(t2) -> ⊨ ⟨t1,t2⟩.fst ⟼⋆ t1.
 Proof.
-  intros k t1 t2 Hvt1 Hvt2; apply multi_step with t1; auto.
+  intros t1 t2 Hvt1 Hvt2; apply multi_step with t1; auto.
 Qed.
 
-Lemma multi_fst1 : forall k t t', k ⊨ t ⟼⋆ t' -> k ⊨ t.fst ⟼⋆ t'.fst.
+Lemma multi_fst1 : forall t t', ⊨ t ⟼⋆ t' -> ⊨ t.fst ⟼⋆ t'.fst.
 Proof.
-  intros k t t' HeT; induction HeT; subst; auto.
+  intros t t' HeT; induction HeT; subst; auto.
   apply multi_step with <[y.fst]>; auto. 
 Qed.
 
-Lemma multi_sndv : forall k t1 t2, value(t1) -> value(t2) -> k ⊨ ⟨t1,t2⟩.snd ⟼⋆ t2.
+Lemma multi_sndv : forall t1 t2, value(t1) -> value(t2) -> ⊨ ⟨t1,t2⟩.snd ⟼⋆ t2.
 Proof.
-  intros k t1 t2 Hvt1 Hvt2; apply multi_step with t2; auto.
+  intros t1 t2 Hvt1 Hvt2; apply multi_step with t2; auto.
 Qed.
 
-Lemma multi_snd1 : forall k t t', k ⊨ t ⟼⋆ t' -> k ⊨ t.snd ⟼⋆ t'.snd.
+Lemma multi_snd1 : forall t t', ⊨ t ⟼⋆ t' -> ⊨ t.snd ⟼⋆ t'.snd.
 Proof.
-  intros k t t' HeT; induction HeT; subst; auto.
+  intros t t' HeT; induction HeT; subst; auto.
   apply multi_step with <[y.snd]>; auto. 
 Qed.
 
-Lemma multi_arr : forall k t t', k ⊨ t ⟼⋆ t' -> k ⊨ arr(t) ⟼⋆ arr(t').
+Lemma multi_arr : forall t t', ⊨ t ⟼⋆ t' -> ⊨ arr(t) ⟼⋆ arr(t').
 Proof.
-  intros k t t' HeT; induction HeT; subst; auto.
+  intros t t' HeT; induction HeT; subst; auto.
   apply multi_step with <[arr(y)]>; auto. 
 Qed.
 
-Lemma multi_first : forall k τ t t', k ⊨ t ⟼⋆ t' -> k ⊨ first(τ:t) ⟼⋆ first(τ:t').
+Lemma multi_first : forall τ t t', ⊨ t ⟼⋆ t' -> ⊨ first(τ:t) ⟼⋆ first(τ:t').
 Proof.
-  intros k τ t t' HeT; induction HeT; subst; auto.
+  intros τ t t' HeT; induction HeT; subst; auto.
   apply multi_step with <[first(τ:y)]>; auto. 
 Qed.
 
-Lemma multi_comp1 : forall k t t' t2, k ⊨ t ⟼⋆ t' -> k ⊨ t >>> t2 ⟼⋆ t' >>> t2.
+Lemma multi_comp1 : forall t t' t2, ⊨ t ⟼⋆ t' -> ⊨ t >>> t2 ⟼⋆ t' >>> t2.
 Proof. 
-  intros k t t' t2 HeT; induction HeT; subst; auto.
+  intros t t' t2 HeT; induction HeT; subst; auto.
   apply multi_step with <[y >>> t2]>; auto.
 Qed.
 
-Lemma multi_comp2 : forall k t t' t1, value(t1) -> k ⊨ t ⟼⋆ t' -> k ⊨ t1 >>> t ⟼⋆ t1 >>> t'.
+Lemma multi_comp2 : forall t t' t1, value(t1) -> ⊨ t ⟼⋆ t' -> ⊨ t1 >>> t ⟼⋆ t1 >>> t'.
 Proof. 
-  intros k t t' t1 Hvt HeT; induction HeT; subst; auto.
+  intros t t' t1 Hvt HeT; induction HeT; subst; auto.
   apply multi_step with <[t1 >>> y]>; auto.
-Qed.
-
-Lemma multi_wh1 : forall k t t' t2, k ⊨ t ⟼⋆ t' -> k ⊨ wormhole(t;t2) ⟼⋆ wormhole(t';t2).
-Proof. 
-  intros k t t' t2 HeT; induction HeT; subst; auto.
-  apply multi_step with <[wormhole(y;t2)]>; auto.
-Qed.
-
-Lemma multi_wh2 : forall k t t' t1, 
-  value(t1) -> (S (S k)) ⊨ t ⟼⋆ t' -> k ⊨ wormhole(t1;t) ⟼⋆ wormhole(t1;t').
-Proof. 
-  intros k t t' t1 Hvt HeT; dependent induction HeT; subst; auto.
-  apply multi_step with <[wormhole(t1;y)]>; auto.
 Qed.
 
 
@@ -235,37 +204,28 @@ Qed.
 
 (** *** Value regards of evaluation transition *)
 
-Lemma value_normal : forall k t, value(t) -> normal_form (evaluate k) t.
+Lemma value_normal : forall t, value(t) -> normal_form evaluate t.
 Proof.
-  intros k t H; generalize k; clear k; induction H; intros k [t' ST]; 
+  intros t H; induction H; intros [t' ST]; 
   try (inversion ST; subst; try destruct (IHvalue k); now eauto);
   try (inversion ST; subst; try destruct (IHvalue1 k); now eauto).
-  - destruct (IHvalue2 k). inversion ST; subst.
-    -- exfalso; apply (IHvalue1 k); now exists t1'.
-    -- now exists t'0.
-  - destruct (IHvalue2 k). inversion ST; subst.
-    -- exfalso; apply (IHvalue1 k); now exists t1'.
-    -- now exists t'0.
-  - destruct (IHvalue2 (S (S k))). inversion ST; subst.
-    -- exfalso; apply (IHvalue1 k); now exists i'.
-    -- now exists t'0.
 Qed.
 
-Lemma evaluate_not_value : forall t t' k, k ⊨ t ⟼ t' -> ~ (value(t)).
+Lemma evaluate_not_value : forall t t', ⊨ t ⟼ t' -> ~ (value(t)).
 Proof.
   intros; induction H; unfold not; intro c; inversion c; subst; eauto.
 Qed.
 
 (** *** Transitivity of multiple evaluation steps *)
 
-Lemma multi_trans : forall k, Transitive (multi k).
+Lemma multi_trans : Transitive multi.
 Proof.
-  red; intros k x y z HmeT HmeT'; induction HmeT; try assumption.
+  red; intros x y z HmeT HmeT'; induction HmeT; try assumption.
   eapply multi_step; eauto.
 Qed.
 
-Lemma indexed_trans : forall lb k k' t t' t'',
-lb ⊨ t ⊢ k ⟶ t' -> lb ⊨ t' ⊢ k' ⟶ t'' -> lb ⊨ t ⊢ (k+k') ⟶ t''.
+Lemma indexed_trans : forall k k' t t' t'',
+  ⊨ t ⊢ k ⟶ t' -> ⊨ t' ⊢ k' ⟶ t'' -> ⊨ t ⊢ (k+k') ⟶ t''.
 Proof.
   induction k; intros.
   - simpl; inversion H; subst; auto.
@@ -273,153 +233,83 @@ Proof.
     eapply IHk; eauto.
 Qed.
 
-(** *** Valid *)
-
-Lemma evaluate_preserves_valid_term : forall t t' k,
-  k ⊩ₜₘ t -> k ⊨ t ⟼ t' -> k ⊩ₜₘ t'.
-Proof.
-  intros t; induction t; intros t' k Hvt HeTt; inversion Hvt; inversion HeTt; 
-  subst; auto; try (constructor; fold Term.valid in *; auto).
-  - inversion Hvt; subst; inversion H4; subst. now apply subst_preserves_valid_4.
-  - inversion Hvt; subst. inversion H5; subst; apply subst_preserves_valid_4; auto.
-  - inversion H1; subst; auto.
-  - inversion H1; subst; auto.
-Qed.
-
-Lemma multi_preserves_valid_term : forall k t t',
-  k ⊩ₜₘ t -> k ⊨ t ⟼⋆ t' -> k ⊩ₜₘ t'.
-Proof.
-  intros; induction H0; auto; apply IHmulti.
-  now apply evaluate_preserves_valid_term with (t := x).
-Qed.
-
-Lemma indexed_preserves_valid_term : forall n t t' k,
-  k ⊩ₜₘ t -> k ⊨ t ⊢ n ⟶ t' -> k ⊩ₜₘ t'.
-Proof.
-  intro n; induction n; intros t t' k Hvt Hi.
-  - inversion Hi; subst; assumption.
-  - inversion Hi; subst; apply IHn with (t := y); try assumption.
-    now apply evaluate_preserves_valid_term with (t := t).
-Qed. 
-
-Theorem evaluate_valid_weakening_gen : forall t t' lb lb' k k',
-  lb <= lb' -> k <= lb -> k' <= lb' -> k <= k' -> lb' - lb = k' - k ->
-  lb ⊨ t ⟼ t' -> lb' ⊨ ([⧐ₜₘ k ≤ {k' - k}] t) ⟼ ([⧐ₜₘ k ≤ {k' - k}] t').
-Proof.
-  intros t t' lb lb' k k' Hle1 Hle Hle' Hle2 Heq eT;
-  revert lb' k k' Hle Hle1 Hle2 Hle' Heq; induction eT; 
-  intros lb' k k' Hle Hle1 Hle2 Hle' Heq; simpl; eauto;
-  try (constructor; eauto; now apply Term.shift_value_iff).
-  - rewrite subst_shift_spec_2; auto. rewrite <- Heq. replace (lb + (lb' - lb)) with lb' by lia.
-    constructor; now apply Term.shift_value_iff.
-  - rewrite subst_shift_spec_2; auto. rewrite <- Heq. replace (lb + (lb' - lb)) with lb' by lia.
-    constructor.
-  - constructor; try (now rewrite <- Term.shift_value_iff); apply IHeT; lia.
-Qed.
-
-Theorem multi_evaluate_valid_weakening_gen : forall t t' lb lb' k k',
-  lb <= lb' -> k <= lb -> k' <= lb' -> k <= k' -> lb' - lb = k' - k ->
-  lb ⊨ t ⟼⋆ t' -> lb' ⊨ ([⧐ₜₘ k ≤ {k' - k}] t) ⟼⋆ ([⧐ₜₘ k ≤ {k' - k}] t').
-Proof.
-  intros; induction H4; try now constructor.
-  eapply multi_step with (y := <[[⧐ₜₘ k ≤ {k' - k}] y ]>); auto.
-  eapply evaluate_valid_weakening_gen with (lb := k0); auto.
-Qed.
-
-Theorem indexed_evaluate_valid_weakening_gen : forall t t' lb lb' k k' n,
-  lb <= lb' -> k <= lb -> k' <= lb' -> k <= k' -> lb' - lb = k' - k ->
-  lb ⊨ t ⊢ n ⟶ t' -> lb' ⊨ ([⧐ₜₘ k ≤ {k' - k}] t) ⊢ n ⟶ ([⧐ₜₘ k ≤ {k' - k}] t').
-Proof.
-  intros; induction H4; try now constructor.
-  eapply index_step with (y := <[[⧐ₜₘ k ≤ {k' - k}] y ]>); auto.
-  eapply evaluate_valid_weakening_gen with (lb := lb); auto.
-Qed.
-
 (** *** Determinism *)
 
-Theorem evaluate_deterministic : forall k t t1 t2,
-  k ⊨ t ⟼ t1 -> k ⊨ t ⟼ t2 -> t1 = t2.
+Theorem evaluate_deterministic : forall t t1 t2,
+  ⊨ t ⟼ t1 -> ⊨ t ⟼ t2 -> t1 = t2.
 Proof with eauto.
-  intros k t t' t'' E1 E2; generalize dependent t''.
+  intros t t' t'' E1 E2; generalize dependent t''.
   induction E1; intros t'' E2; inversion E2; subst; try (f_equal; now auto); 
   exfalso; try (eapply value_normal; now eauto); clear E2...
   - eapply value_normal in H...
   - inversion E1; subst.
     -- eapply value_normal in H0...
-    -- eapply value_normal in H2...
-  - inversion H3; subst.
+    -- eapply value_normal in H1...
+  - inversion H2; subst.
     -- eapply value_normal in H...
     -- eapply value_normal in H0...
   - inversion E1; subst.
     -- eapply value_normal in H0...
-    -- eapply value_normal in H2...
-  - inversion H3; subst.
+    -- eapply value_normal in H1...
+  - inversion H2; subst.
     -- eapply value_normal in H...
     -- eapply value_normal in H0...
 Qed.
 
-Theorem indexed_deterministic : forall n k t t1 t2,
-  k ⊨ t ⊢ n ⟶ t1 -> k ⊨ t ⊢ n ⟶ t2 -> t1 = t2.
+Theorem indexed_deterministic : forall n t t1 t2,
+  ⊨ t ⊢ n ⟶ t1 -> ⊨ t ⊢ n ⟶ t2 -> t1 = t2.
 Proof.
-intros n; induction n; intros k t t1 t2 Hev1 Hev2.
+intros n; induction n; intros t t1 t2 Hev1 Hev2.
 - inversion Hev1; inversion Hev2; subst; reflexivity.
 - inversion Hev1; inversion Hev2; subst.
-  apply evaluate_deterministic with (t1 := y) in H6; auto; subst. 
-  now apply IHn with (k := k) (t := y0).
+  apply evaluate_deterministic with (t1 := y) in H5; auto; subst. 
+  now apply IHn with (t := y0).
 Qed.
 
 
 (** *** Halts *)
 
-Lemma value_halts : forall k t, value(t) -> halts k t.
+Lemma value_halts : forall t, value(t) -> halts t.
 Proof. 
-  intros k t Hv; unfold halts; exists t; split; try assumption.
+  intros t Hv; unfold halts; exists t; split; try assumption.
   apply multi_refl.
 Qed.
 
-Lemma evaluate_preserves_halting : forall k t t',
-  k ⊨ t ⟼ t' -> (halts k t <-> halts k t').
+Lemma evaluate_preserves_halting : forall t t',
+  ⊨ t ⟼ t' -> (halts t <-> halts t').
 Proof.
-  intros k t t' HeT; unfold halts; split; intros [t'' [HmeT Hv]].
+  intros t t' HeT; unfold halts; split; intros [t'' [HmeT Hv]].
   - destruct HmeT.
-    -- exfalso; apply (value_normal k) in Hv; unfold normal_form,not in Hv; apply Hv.
+    -- exfalso; apply value_normal in Hv; unfold normal_form,not in Hv; apply Hv.
       now exists t'.
-    -- apply (evaluate_deterministic k x t' y HeT) in H as Heq; subst.
+    -- apply (evaluate_deterministic x t' y HeT) in H as Heq; subst.
       exists z; split; assumption.
   - exists t''; split; try assumption; now apply multi_step with (y := t').     
 Qed.
 
-Lemma multi_preserves_halting : forall k t t',
-  k ⊨ t ⟼⋆ t' -> (halts k t <-> halts k t').
+Lemma multi_preserves_halting : forall t t',
+  ⊨ t ⟼⋆ t' -> (halts t <-> halts t').
 Proof.
-  intros k t t' HmeT; induction HmeT; unfold halts; split; intros [t'' [HmeT' Hv]];
+  intros t t' HmeT; induction HmeT; unfold halts; split; intros [t'' [HmeT' Hv]];
   try (exists t''; now split).
   - apply evaluate_preserves_halting in H as H'.
-    assert (halts k x). { exists t''; now split. }
+    assert (halts x). { exists t''; now split. }
     rewrite H' in H0; now rewrite IHHmeT in H0.
   - apply evaluate_preserves_halting in H as H'.
-    assert (halts k z). { exists t''; now split. }
+    assert (halts z). { exists t''; now split. }
     rewrite <- IHHmeT in H0. now rewrite <- H' in H0.
 Qed.
 
-Lemma halts_weakening : forall k k' t, k <= k' -> halts k t -> halts k' <[[⧐ₜₘ k ≤ {k' - k}] t]>.
+Lemma halts_pair : forall t1 t2,
+  halts <[⟨t1,t2⟩]> <-> halts t1 /\ halts t2.
 Proof.
-  unfold halts; intros. destruct H0 as [t' [HeT Hvt']].
-  exists <[[⧐ₜₘ k ≤ {k' - k}] t']>; split.
-  - eapply multi_evaluate_valid_weakening_gen; eauto.
-  - now apply Term.shift_value_iff.
-Qed.
-
-Lemma halts_pair : forall k t1 t2,
-  halts k <[⟨t1,t2⟩]> <-> halts k t1 /\ halts k t2.
-Proof.
-  assert (Hpair : forall k t1 t2 t, k ⊨ ⟨t1,t2⟩ ⟼⋆ t -> exists t1' t2', t = <[⟨t1',t2'⟩]>).
+  assert (Hpair : forall t1 t2 t, ⊨ ⟨t1,t2⟩ ⟼⋆ t -> exists t1' t2', t = <[⟨t1',t2'⟩]>).
   {
-    intros k t1 t2 t HeT; dependent induction HeT; subst.
+    intros t1 t2 t HeT; dependent induction HeT; subst.
     - exists t1; now exists t2.
     - inversion H; subst; eauto. 
   }
-  intros k t1 t2; split; intros HA.
+  intros t1 t2; split; intros HA.
   - destruct HA as [t [HmeT Hvt]]. apply Hpair in HmeT as Heq.
     destruct Heq as [t1' [t2' Heq]]; subst. dependent induction HmeT.
     -- inversion Hvt; subst; split.
@@ -444,17 +334,17 @@ Qed.
 
 (** *** Relation between eval,multi and indexed transition *)
 
-Lemma evaluate_indexed_1_iff : forall k t t',
-  k ⊨ t ⟼ t' <-> k ⊨ t ⊢ 1 ⟶ t'.
+Lemma evaluate_indexed_1_iff : forall t t',
+  ⊨ t ⟼ t' <-> ⊨ t ⊢ 1 ⟶ t'.
 Proof.
   split; intros.
   - replace 1 with (0 + 1); eauto; 
     eapply index_step; eauto; apply index_refl; auto.
-  - inversion H; subst. inversion H3; subst; auto.
+  - inversion H; subst. inversion H2; subst; auto.
 Qed.
 
-Lemma multi_indexed : forall lb t t',
-  lb ⊨ t ⟼⋆ t' -> exists k, lb ⊨ t ⊢ k ⟶ t'.
+Lemma multi_indexed : forall t t',
+  ⊨ t ⟼⋆ t' -> exists k, ⊨ t ⊢ k ⟶ t'.
 Proof.
   intros. induction H.
   - exists 0. apply index_refl; auto.
@@ -463,88 +353,52 @@ Qed.
 
 (** ** Preservation *)
 
-(** *** Proof of preservation of typing through the evaluation transition
-
-  **** Hypothesis
-
-  Knowing the context is valid regards of its own new key (1),
-  the term t is well typed according to a certain context Re (2), 
-  there is a certain t' that is the result of t after one step of transition (3);
-
-  **** Result
-
-  We can state that the term t' is well typed. 
-*)
+(** *** Proof of preservation of typing through an evaluation transition *)
 Theorem evaluate_preserves_typing : forall Re t t' τ,
-  (* (1) *) newᵣᵪ(Re) ⊩ᵣᵪ Re ->
-  (* (2) *) ∅ᵥᵪ ⋅ Re ⊫ t ∈ τ -> 
-  (* (3) *) (newᵣᵪ(Re)) ⊨ t ⟼ t' -> 
+  ∅ᵥᵪ ⋅ Re ⊫ t ∈ τ -> ⊨ t ⟼ t' -> 
 
   ∅ᵥᵪ ⋅ Re ⊫ t' ∈ τ.
 Proof. 
-  intros Re t t' τ HvRe Hwt; generalize dependent t'; dependent induction Hwt; intros t' HeTt;
+  intros Re t t' τ Hwt; generalize dependent t'; dependent induction Hwt; intros t' HeTt;
   inversion HeTt; subst; try (econstructor; now eauto); eauto.
-  - inversion Hwt1; subst. eapply subst_preserves_typing; eauto.
+  - inversion Hwt1; subst. eapply subst_preserves_typing; eauto. apply RContext.Submap_refl.
   - inversion Hwt2; subst; inversion Hwt1.
   - inversion Hwt; subst; auto.
   - inversion Hwt; subst; auto.
   - inversion Hwt; subst. eapply subst_preserves_typing; eauto. constructor; eauto.
-  - econstructor; eauto. apply IHHwt2; auto.
-    -- rewrite RContext.new_key_wh_spec; apply RContext.valid_wh_spec; auto;
-        unfold Typ.PairTyp.valid; simpl; split; try (constructor);
-        apply well_typed_implies_valid in Hwt1 as [_ Hvτ]; auto; apply VContext.valid_empty_spec.
-    -- now rewrite RContext.new_key_wh_spec.
+    apply RContext.Submap_refl.
 Qed.
 
-(** *** Proof of preservation of typing through multiple evaluation transitions
-
-  **** Hypothesis
-
-  Knowing the context is valid regards of its own new key (1),
-  the term t is well typed according to a certain context Re (2), 
-  there is a certain t' that is the result of t after zero or k steps of transition (3);
-
-  **** Result
-
-  We can state that the term t' is well typed. 
-*)
+(** *** Proof of preservation of typing through multiple evaluation transitions *)
 Theorem multi_preserves_typing : forall Re t t' τ,
-  (* (1) *) newᵣᵪ(Re) ⊩ᵣᵪ Re ->
-  (* (2) *) ∅ᵥᵪ ⋅ Re ⊫ t ∈ τ -> 
-  (* (3) *) (newᵣᵪ(Re)) ⊨ t ⟼⋆ t' -> 
+  ∅ᵥᵪ ⋅ Re ⊫ t ∈ τ -> ⊨ t ⟼⋆ t' -> 
   
   ∅ᵥᵪ ⋅ Re ⊫ t' ∈ τ.
 Proof.
-  intros Re t t' τ HvRe Hwt HmeT; dependent induction HmeT; subst; try assumption.
-  apply IHHmeT; auto. eapply (evaluate_preserves_typing Re x y τ HvRe Hwt H).
+  intros Re t t' τ Hwt HmeT; dependent induction HmeT; subst; try assumption.
+  apply IHHmeT; auto. eapply (evaluate_preserves_typing Re x y τ Hwt H).
 Qed.
 
 (** ** Progress *)
 
-(** *** Proof of progress of the evaluation transtion
-
-  If the term is well typed then 
-  - either we have a value (1) or 
-  - we can evaluate at least one time the term (2).
-
-*)
+(** *** Proof of progress of the evaluation transtion *)
 Theorem progress_of_evaluate : forall t Re τ,
   ∅ᵥᵪ ⋅ Re ⊫ t ∈ τ -> 
   
   (* (1) *) value(t) \/ 
-  (* (2) *) exists t', (newᵣᵪ(Re)) ⊨ t ⟼ t'.
+  (* (2) *) exists t', ⊨ t ⟼ t'.
 Proof.
   intro t; induction t; intros Re τ' Hwt; inversion Hwt; subst; 
   try (now left); try (apply IHt1 in H3 as H3'; apply IHt2 in H5 as H5').
   - destruct H3',H5'; right. 
-    -- inversion H; subst; inversion H3; subst. exists <[[x:= t2 ~ {newᵣᵪ(Re)} ≤ 0] t]>.
+    -- inversion H; subst; inversion H3; subst. exists <[[x:= t2] t]>.
       now constructor.
     -- destruct H0; exists <[t1 x]>; now constructor.
     -- destruct H; exists <[x t2]>; now constructor.
     -- destruct H; exists <[x t2]>; now constructor.
   - right; apply IHt2 in H4 as H4'; destruct H4'.
     -- destruct t2; inversion H4; subst; inversion H; subst.
-        exists <[[v := Fix (\ v : τ', t2) ~ {newᵣᵪ(Re)} ≤ 0] t2]>; constructor.
+        exists <[[v := Fix (\ v : τ', t2)] t2]>; constructor.
     -- destruct H; exists <[Fix x]>; constructor; auto.
   - destruct H3',H5'; auto.
     -- right; destruct H0; exists <[⟨t1,x⟩]>; now constructor.
@@ -558,7 +412,7 @@ Proof.
     -- destruct H; exists (Term.tm_snd x); now constructor.
   - apply IHt in H2 as H2'; destruct H2' as [Hvt | [t' HeT']]; 
     try (left; now constructor); right; exists <[arr(t')]>; now constructor.
-  - apply IHt in H3 as H3'; destruct H3' as [Hvt | [t' HeT']]; 
+  - apply IHt in H4 as H4'; destruct H4' as [Hvt | [t' HeT']]; 
     try (left; now constructor); right; exists <[first(τ:t')]>; now constructor.
   - apply IHt1 in H1 as H1'; apply IHt2 in H5 as H5';
     destruct H1' as [Hvt1 | [t1' HeT1']]; destruct H5' as [Hvt2 | [t2' HeT2']];
@@ -566,28 +420,4 @@ Proof.
     -- exists <[t1 >>> t2']>; now constructor.
     -- exists <[t1' >>> t2]>; now constructor.
     -- exists <[t1' >>> t2]>; now constructor.
-  - apply IHt1 in H1 as H1'; apply IHt2 in H8 as H8';
-    destruct H1' as [Hvt1 | [t1' HeT1']]; destruct H8' as [Hvt2 | [t2' HeT2']];
-    try (left; now constructor); right.
-    -- exists <[wormhole(t1;t2')]>; constructor; auto.
-        unfold k in HeT2'; rewrite RContext.new_key_wh_spec in HeT2'; auto.
-    -- exists <[wormhole(t1';t2)]>; now constructor.
-    -- exists <[wormhole(t1';t2)]>; now constructor.
 Qed.
-
-(** *** Some corollaries *)  
-
-Corollary evaluate_valid_weakening : forall t t' k k',
-  k <= k' ->
-  k ⊨ t ⟼ t' -> k' ⊨ ([⧐ₜₘ k ≤ {k' - k}] t) ⟼ ([⧐ₜₘ k ≤ {k' - k}] t').
-Proof. intros. apply evaluate_valid_weakening_gen with (lb := k); eauto. Qed.
-
-Corollary multi_evaluate_valid_weakening : forall t t' k k',
-  k <= k' ->
-  k ⊨ t ⟼⋆ t' -> k' ⊨ ([⧐ₜₘ k ≤ {k' - k}] t) ⟼⋆ ([⧐ₜₘ k ≤ {k' - k}] t').
-Proof. intros; apply multi_evaluate_valid_weakening_gen with (lb := k); auto. Qed.
-
-Corollary indexed_evaluate_valid_weakening : forall t t' k k' n,
-  k <= k' ->
-  k ⊨ t ⊢ n ⟶ t' -> k' ⊨ ([⧐ₜₘ k ≤ {k' - k}] t) ⊢ n ⟶ ([⧐ₜₘ k ≤ {k' - k}] t').
-Proof. intros; apply indexed_evaluate_valid_weakening_gen with (lb := k); auto. Qed.
